theories/aneris_lang/state_interp/state_interp_config_wp.v
@@ -32,13 +32,9 @@ Section state_interpretation.
 
   Lemma config_wp_correct : ⊢ config_wp.
   Proof.
-    rewrite /config_wp.
-    iIntros.
-    iModIntro.
-    iIntros (σ1 δ k σ2 ks nt Hstep) "Hst".
+    rewrite /config_wp. iIntros. iModIntro. iIntros (σ1 δ k σ2 ks nt Hstep) "Hσ".
     rewrite /state_interp; simplify_eq /=.
-    iDestruct "Hst"
-      as (γm)
+    iDestruct "Hσ" as (γm)
            "(%Hgcoh & %Hnscoh & %Hmhcoh
                     & Hnauth & Hsi & Hlcoh & Hfreeips & Hmctx & Hmres)".
     iApply step_fupd_fupd; iApply step_fupd_intro; first done.
@@ -46,32 +42,25 @@ Section state_interpretation.
         [ ip σ k Sn Sn' sh a skt R m Hm HSn Hsh HSn' Hsaddr | σ]; simpl.
     { iExists δ. iIntros "!> !>". iSplit.
       - iPureIntro. split_and!; last by left.
-        simplify_eq. admit.
+        simplify_eq. eapply message_history_evolution_deliver_message; eauto.
+        edestruct Hnscoh as (?&?&?&Hac&?); first done. by symmetry; eapply Hac.
       - iExists γm. iFrame "Hsi".
         iSplitR; [eauto using gnames_coh_update_sockets|].
         iSplitR; [eauto using network_sockets_coh_deliver_message|].
         iSplitR; [eauto using messages_history_coh_deliver_message|].
-        iFrame.
-        iSplitL "Hlcoh".
+        iFrame. iSplitL "Hlcoh".
         + by iApply (local_state_coh_deliver_message with "[Hlcoh]").
-        + iSplitL "Hfreeips".
-            by iApply free_ips_coh_deliver_message.
-            rewrite /messages_resource_coh.
-            iApply (big_sepS_mono with "Hmres").
-            iIntros (??) "[Hmr|%Hmr]"; last eauto with iFrame.
-            iLeft. iDestruct "Hmr" as (phi) "(Hphi & Hphi2)".
-            eauto with iFrame. }
-    iExists δ. iIntros "!> !>". iSplit.
-    iPureIntro. split_and!; last by left.
-    simplify_eq. admit.
-    iExists γm. iFrame.
-    iSplitR; first done.
-    iSplitR; first done.
+        + iSplitL "Hfreeips". by iApply free_ips_coh_deliver_message.
+          rewrite /messages_resource_coh. iApply (big_sepS_mono with "Hmres").
+          iIntros (??) "[Hmr|%Hmr]"; last eauto with iFrame. iLeft.
+          iDestruct "Hmr" as (phi) "(Hphi & Hphi2)". eauto with iFrame. }
+    iExists δ. iIntros "!> !>". iSplit. iPureIntro. split_and!; last by left.
+    simplify_eq. by eapply message_history_evolution_drop_message.
+    iExists γm. iFrame. iSplitR; first done. iSplitR; first done.
     iSplitR. iPureIntro. simpl. by eapply messages_history_drop_message.
-    rewrite /messages_resource_coh.
-    iApply (big_sepS_mono with "Hmres").
-    iIntros (??) "[Hmr|%Hmr]"; last eauto with iFrame.
-    iLeft. iDestruct "Hmr" as (phi) "(Hphi & Hphi2)". eauto with iFrame.
-    Admitted.
+    rewrite /messages_resource_coh. iApply (big_sepS_mono with "Hmres").
+    iIntros (??) "[Hmr|%Hmr]"; last eauto with iFrame. iLeft.
+    iDestruct "Hmr" as (phi) "(Hphi & Hphi2)". eauto with iFrame.
+  Qed.
 
 End state_interpretation.
